thy/Bitmagic/Numberwang_Ln.thy
@@ -2,10 +2,10 @@ theory Numberwang_Ln
 imports NumberWangCebewee
 begin
 
-lemma ipv4range_bitmask_intersect: " \<not> ipv4range_set_from_bitmask b2 m2 \<subseteq> ipv4range_set_from_bitmask b1 m1 \<Longrightarrow>
-       \<not> ipv4range_set_from_bitmask b1 m1 \<subseteq> ipv4range_set_from_bitmask b2 m2 \<Longrightarrow>
-       ipv4range_set_from_bitmask b1 m1 \<inter> ipv4range_set_from_bitmask b2 m2 = {}"
-apply(simp add: ipv4range_set_from_bitmask_eq_ip4_set)
+lemma ipv4range_prefix_intersect: " \<not> ipv4range_set_from_prefix b2 m2 \<subseteq> ipv4range_set_from_prefix b1 m1 \<Longrightarrow>
+       \<not> ipv4range_set_from_prefix b1 m1 \<subseteq> ipv4range_set_from_prefix b2 m2 \<Longrightarrow>
+       ipv4range_set_from_prefix b1 m1 \<inter> ipv4range_set_from_prefix b2 m2 = {}"
+apply(simp add: ipv4range_set_from_prefix_eq_ip4_set)
 using ip4_set_notsubset_empty_inter by presburger
 
 
